Refactored atomic exchange, verified spinlocks on top of it.

progs/mailbox.c
@@ -1,6 +1,6 @@
 #include <stdlib.h>
 #include <stdio.h>
-#include "threads.h"
+#include "atomic_exchange.h"
 
 void *surely_malloc (size_t n) {
   void *p = malloc(n);
@@ -27,16 +27,6 @@ typedef struct buffer {int data;} buffer;
 buffer *bufs[B];
 lock_t *lock[N];
 buf_id *comm[N];
-
-//This could be replaced by an external call.
-int simulate_atomic_exchange(int *tgt, lock_t *l, int v){
-  int x;
-  acquire(l);
-  x = *tgt;
-  *tgt = v;
-  release(l);
-  return x;
-}
 
 //The initial state as written in the draft is slightly inconsistent:
 //last_read is First, but comm[r] is also First as if it
