progs/verif_atomic_exchange.v
@@ -1,0 +1,236 @@
+Require Import veric.rmaps.
+Require Import progs.conclib.
+Require Import progs.ghost.
+Require Import floyd.library.
+Require Import floyd.sublist.
+Require Import progs.atomic_exchange.
+
+Set Bullet Behavior "Strict Subproofs".
+
+Instance CompSpecs : compspecs. make_compspecs prog. Defined.
+Definition Vprog : varspecs. mk_varspecs prog. Defined.
+
+Definition acquire_spec := DECLARE _acquire acquire_spec.
+Definition release_spec := DECLARE _release release_spec.
+
+Definition hist := AE_hist.
+
+Definition AE_inv x i sh R := EX h : list AE_hist_el, EX v : val,
+  !!(apply_hist i h = Some v /\ tc_val tint v) &&
+  (data_at sh tint v x * ghost ([] : hist, Some h) x * R h v * (weak_precise_mpred (R h v) && emp)).
+
+Lemma AE_inv_positive : forall x i sh R, readable_share sh -> positive_mpred (AE_inv x i sh R).
+Proof.
+  unfold AE_inv; intros.
+  do 2 (apply ex_positive; intro).
+  apply positive_andp2, positive_sepcon1, positive_sepcon1, positive_sepcon1; auto.
+Qed.
+Hint Resolve AE_inv_positive.
+
+Lemma AE_inv_precise : forall x i sh R (Hsh : readable_share sh),
+  predicates_hered.derives TT (weak_precise_mpred (AE_inv x i sh R)).
+Proof.
+  intros ????? rho _ ???
+    (? & h1 & v1 & (Hh1 & ?) & ? & ? & Hj1 & (? & r1 & Hj'1 & (? & ? & ? & (? & Hv1) & Hg1) & HR1) & (HR & Hemp1))
+    (? & h2 & v2 & (Hh2 & ?) & ? & ? & Hj2 & (? & r2 & Hj'2 & (? & ? & ? & (? & Hv2) & Hg2) & HR2) & (_ & Hemp2))
+    Hw1 Hw2.
+  unfold at_offset in *; simpl in *; rewrite data_at_rec_eq in Hv1, Hv2; simpl in *.
+  exploit (mapsto_inj _ _ _ _ _ _ _ w Hsh Hv1 Hv2); auto; try join_sub; unfold unfold_reptype; simpl.
+  { intro; subst; contradiction. }
+  { intro; subst; contradiction. }
+  intros (? & Hv); subst.
+  exploit (ghost_inj _ _ _ _ _ w Hg1 Hg2); try join_sub.
+  intros (? & Heq); inv Heq.
+  destruct (age_sepalg.join_level _ _ _ Hj1), (age_sepalg.join_level _ _ _ Hj2),
+    (age_sepalg.join_level _ _ _ Hj'1), (age_sepalg.join_level _ _ _ Hj'2).
+  pose proof (juicy_mem.rmap_join_sub_eq_level _ _ Hw1);
+    pose proof (juicy_mem.rmap_join_sub_eq_level _ _ Hw2).
+  exploit (HR w r1 r2); try (split; auto; omega); try join_sub.
+  intro; subst; join_inj.
+  apply sepalg.join_comm in Hj1; apply sepalg.join_comm in Hj2.
+  match goal with H1 : predicates_hered.app_pred emp ?a,
+    H2 : predicates_hered.app_pred emp ?b |- _ => assert (a = b);
+      [eapply sepalg.same_identity; auto;
+        [match goal with H : sepalg.join a ?x ?y |- _ =>
+           specialize (Hemp1 _ _ H); instantiate (1 := x); subst; auto end |
+         match goal with H : sepalg.join b ?x ?y |- _ =>
+           specialize (Hemp2 _ _ H); subst; auto end] | subst] end.
+  join_inj.
+Qed.
+
+(* Can we always provide a clunky function such that P and Q are a single function? *)
+(* Compare and contrast with magic wand proof of bin tree *)
+Definition AE_spec i P R Q := forall hc hx vc vx (Hvx : apply_hist i hx = Some vx) (Hhist : hist_incl _ hc hx),
+  view_shift (R hx vx * P hc vc)
+  (R (hx ++ [AE vx vc]) vc * (weak_precise_mpred (R (hx ++ [AE vx vc]) vc) && emp) *
+   Q (hc ++ [(length hx, AE vx vc)]) vx).
+
+Definition AE_type := ProdType (ProdType (ProdType
+  (ConstType (share * share * val * val * val * val * hist))
+  (ArrowType (ConstType hist) (ArrowType (ConstType val) Mpred)))
+  (ArrowType (ConstType (list AE_hist_el)) (ArrowType (ConstType val) Mpred)))
+  (ArrowType (ConstType hist) (ArrowType (ConstType val) Mpred)).
+
+Notation "'TYPE' A 'WITH'  x1 : t1 , x2 : t2 , x3 : t3 , x4 : t4 , x5 : t5 , x6 : t6 , x7 : t7 , x8 : t8 , x9 : t9 , x10 : t10 'PRE'  [ u , .. , v ] P 'POST' [ tz ] Q" :=
+     (mk_funspec ((cons u%formals .. (cons v%formals nil) ..), tz) cc_default A
+  (fun (ts: list Type) (x: t1*t2*t3*t4*t5*t6*t7*t8*t9*t10) =>
+     match x with (x1,x2,x3,x4,x5,x6,x7,x8,x9,x10) => P%assert end)
+  (fun (ts: list Type) (x: t1*t2*t3*t4*t5*t6*t7*t8*t9*t10) =>
+     match x with (x1,x2,x3,x4,x5,x6,x7,x8,x9,x10) => Q%assert end) _ _)
+            (at level 200, x1 at level 0, x2 at level 0, x3 at level 0, x4 at level 0, 
+             x5 at level 0, x6 at level 0, x7 at level 0, x8 at level 0, x9 at level 0, x10 at level 0,
+             P at level 100, Q at level 100).
+
+Definition ghost_hist (h : hist) p := ghost (h, @None (list AE_hist_el)) p.
+
+(* It would be nice to be able to store any kind of data in the location, but that won't typecheck. *)
+Program Definition atomic_exchange_spec := DECLARE _simulate_atomic_exchange
+  TYPE AE_type WITH ish : share, lsh : share, tgt : val, l : val,
+    i : val, v : val, h : hist, P : hist -> val -> mpred, R : list AE_hist_el -> val -> mpred, Q : hist -> val -> mpred
+  PRE [ _tgt OF tptr tint, _l OF tptr (Tstruct _lock_t noattr), _v OF tint ]
+   PROP (tc_val tint v; readable_share lsh; writable_share ish; AE_spec i P R Q)
+   LOCAL (temp _tgt tgt; temp _l l; temp _v v)
+   SEP (lock_inv lsh l (AE_inv tgt i ish R); ghost_hist h tgt; P h v)
+  POST [ tint ]
+   EX t : nat, EX v' : val,
+   PROP (tc_val tint v'; Forall (fun x => fst x < t)%nat h)
+   LOCAL (temp ret_temp v')
+   SEP (lock_inv lsh l (AE_inv tgt i ish R); ghost_hist (h ++ [(t, AE v' v)]) tgt;
+        Q (h ++ [(t, AE v' v)]) v').
+Next Obligation.
+Proof.
+  replace _ with (fun (_ : list Type)
+    (x : share * share * val * val * val * val * hist *
+         (hist -> val -> mpred) * (list AE_hist_el -> val -> mpred) * (hist -> val -> mpred)) rho =>
+    PROP (let '(ish, lsh, tgt, l, i, v, h, P, R, Q) := x in tc_val tint v /\ readable_share lsh /\
+      writable_share ish /\ AE_spec i P R Q)
+    LOCAL (let '(ish, lsh, tgt, l, i, v, h, P, R, Q) := x in temp _tgt tgt;
+           let '(ish, lsh, tgt, l, i, v, h, P, R, Q) := x in temp _l l;
+           let '(ish, lsh, tgt, l, i, v, h, P, R, Q) := x in temp _v v)
+    SEP (let '(ish, lsh, tgt, l, i, v, h, P, R, Q) := x in
+         lock_inv lsh l (AE_inv tgt i ish R) * ghost_hist h tgt * P h v) rho).
+  apply (PROP_LOCAL_SEP_super_non_expansive AE_type [fun _ => _] [fun _ => _; fun _ => _; fun _ => _]
+    [fun _ => _]); repeat constructor; hnf; intros;
+    destruct x as (((((((((?, ?), ?), ?), ?), ?), ?), P), R), Q); auto; simpl.
+  - unfold AE_spec.
+    (* This is probably provable for derives, but might need to be assumed for view shift. *)
+    admit.
+  - rewrite !approx_sepcon.
+    replace (compcert_rmaps.RML.R.approx n (P h v2)) with
+      (base.compose (compcert_rmaps.R.approx n) (compcert_rmaps.R.approx n) (P h v2)) at 1
+      by (rewrite compcert_rmaps.RML.approx_oo_approx; auto).
+    evar (rhs : mpred); replace (compcert_rmaps.RML.R.approx _ _) with rhs; subst rhs; [reflexivity|].
+    rewrite (nonexpansive_super_non_expansive (fun R => lock_inv s0 v0 R)); [|apply nonexpansive_lock_inv].
+    setoid_rewrite (nonexpansive_super_non_expansive (fun R => lock_inv s0 v0 R)) at 2; [|apply nonexpansive_lock_inv].
+    f_equal; f_equal.
+    unfold AE_inv; rewrite !approx_exp; f_equal; extensionality l'.
+    rewrite !approx_exp; f_equal; extensionality z'.
+    rewrite !approx_andp, !approx_sepcon; f_equal; f_equal.
+    * replace (compcert_rmaps.RML.R.approx n (R l' z')) with
+        (base.compose (compcert_rmaps.R.approx n) (compcert_rmaps.R.approx n) (R l' z')) at 2
+        by (rewrite compcert_rmaps.RML.approx_oo_approx; auto); auto.
+    * rewrite !approx_andp; f_equal.
+      setoid_rewrite nonexpansive_super_non_expansive at 2; [|apply precise_mpred_nonexpansive]; auto.
+  - extensionality ts x rho.
+    destruct x as (((((((((?, ?), ?), ?), ?), ?), ?), P), R), Q); auto.
+    unfold PROPx, SEPx; simpl; rewrite !sepcon_assoc; f_equal.
+    f_equal; apply prop_ext; tauto.
+Admitted.
+Next Obligation.
+Proof.
+  replace _ with (fun (_ : list Type)
+    (x : share * share * val * val * val * val * hist *
+         (hist -> val -> mpred) * (list AE_hist_el -> val -> mpred) * (hist -> val -> mpred)) rho =>
+    EX t : nat, EX v' : val,
+      PROP (let '(ish, lsh, tgt, l, i, v, h, P, R, Q) := x in
+            tc_val tint v' /\ Forall (fun x => (fst x < t)%nat) h)
+      LOCAL (let '(ish, lsh, tgt, l, i, v, h, P, R, Q) := x in temp ret_temp v')
+      SEP (let '(ish, lsh, tgt, l, i, v, h, P, R, Q) := x in
+           lock_inv lsh l (AE_inv tgt i ish R) * ghost_hist (h ++ [(t, AE v' v)]) tgt *
+           Q (h ++ [(t, AE v' v)]) v') rho).
+  repeat intro.
+  rewrite !approx_exp; f_equal; extensionality t.
+  rewrite !approx_exp; f_equal; extensionality v'.
+  pose proof (PROP_LOCAL_SEP_super_non_expansive AE_type
+    [fun ts x => let '(_, _, _, _, _, _, h, _, _, _) := x in tc_val tint v' /\ Forall (fun x => (fst x < t)%nat) h]
+    [fun ts x => let '(_, _, _, _, _, _, _, _, _, _) := x in temp ret_temp v']
+    [fun ts x => let '(ish, lsh, tgt, l, i, v, h, P, R, Q) := x in
+       lock_inv lsh l (AE_inv tgt i ish R) * ghost_hist (h ++ [(t, AE v' v)]) tgt *
+       Q (h ++ [(t, AE v' v)]) v'])
+    as Heq; apply Heq; repeat constructor; hnf; intros;
+      destruct x0 as (((((((((?, ?), ?), ?), ?), ?), ?), P), R), Q); auto; simpl.
+  - rewrite !approx_sepcon; f_equal.
+    + rewrite (nonexpansive_super_non_expansive (fun R => lock_inv s0 v0 R)); [|apply nonexpansive_lock_inv].
+      f_equal.
+      setoid_rewrite (nonexpansive_super_non_expansive (fun R => lock_inv s0 v0 R)) at 2; [|apply nonexpansive_lock_inv].
+      f_equal; f_equal.
+      unfold AE_inv; rewrite !approx_exp; f_equal; extensionality l'.
+      rewrite !approx_exp; f_equal; extensionality z'.
+      rewrite !approx_andp, !approx_sepcon; f_equal; f_equal.
+      * replace (compcert_rmaps.RML.R.approx n0 (R l' z')) with
+          (base.compose (compcert_rmaps.R.approx n0) (compcert_rmaps.R.approx n0) (R l' z')) at 1
+          by (rewrite compcert_rmaps.RML.approx_oo_approx; auto); auto.
+      * rewrite !approx_andp; f_equal.
+        apply (nonexpansive_super_non_expansive), precise_mpred_nonexpansive.
+    + replace (compcert_rmaps.RML.R.approx n0 (Q _ v')) with
+        (base.compose (compcert_rmaps.R.approx n0) (compcert_rmaps.R.approx n0) (Q (h ++ [(t, AE v' v2)]) v')) at 1
+        by (rewrite compcert_rmaps.RML.approx_oo_approx; auto); auto.
+  - extensionality ts x rho.
+    destruct x as (((((((((?, ?), ?), ?), ?), ?), ?), P), R), Q); auto.
+    f_equal; extensionality.
+    f_equal; extensionality.
+    unfold PROPx, SEPx; simpl; rewrite !sepcon_assoc; f_equal.
+    f_equal; apply prop_ext; tauto.
+Qed.
+
+Definition Gprog : funspecs := ltac:(with_library prog [acquire_spec; release_spec; atomic_exchange_spec]).
+
+Lemma body_atomic_exchange : semax_body Vprog Gprog f_simulate_atomic_exchange atomic_exchange_spec.
+Proof.
+  start_dep_function.
+  simpl; destruct ts as (((((((((ish, lsh), tgt), l), i), v), h), P), R), Q).
+  rewrite lock_inv_isptr; Intros.
+  forward_call (l, lsh, AE_inv tgt i ish R).
+  unfold AE_inv at 2; Intros h' v'.
+  gather_SEP 2 5; rewrite sepcon_comm.
+  assert_PROP (join (h, None) ([], Some h') (h, Some h')) as Hjoin.
+  { go_lowerx; apply sepcon_derives_prop.
+    eapply derives_trans; [apply ghost_conflict|].
+    apply prop_left; intros (? & (_ & Hh) & ([(? & ?) | (<- & _)] & Hincl)); try discriminate; simpl in *.
+    apply prop_right; rewrite app_nil_r in *; repeat split; auto.
+    repeat intro; apply Hincl.
+    rewrite <- Hh; auto. }
+  unfold ghost_hist; rewrite (ghost_join _ _ _ _ Hjoin).
+  forward.
+  forward.
+  assert (apply_hist i (h' ++ [AE v' v]) = Some v) as Hh'.
+  { rewrite apply_hist_app.
+    replace (apply_hist i h') with (Some v'); simpl.
+    apply eq_dec_refl. }
+  apply hist_add with (e := AE v' v).
+  destruct Hjoin as (? & ? & Hincl); simpl in Hincl.
+  erewrite <- ghost_join; [|apply hist_sep_join].
+  gather_SEP 3 5; simpl.
+  match goal with H : AE_spec _ _ _ _ |- _ => apply H; auto end.
+  forward_call (l, lsh, AE_inv tgt i ish R).
+  { rewrite ?sepcon_assoc; rewrite <- sepcon_emp at 1; rewrite sepcon_comm; apply sepcon_derives;
+      [repeat apply andp_right; auto; eapply derives_trans; try apply positive_weak_positive; auto|].
+    { apply AE_inv_precise; auto. }
+    unfold AE_inv.
+    Exists (h' ++ [AE v' v]) v; entailer!.
+    cancel.
+    rewrite (sepcon_comm (_ * _) (ghost _ _)), !sepcon_assoc; apply sepcon_derives; auto; cancel. }
+  forward.
+  Exists (length h') (Vint v'); entailer!.
+  - rewrite Forall_forall; intros (?, ?) Hin.
+    specialize (Hincl _ _ Hin).
+    simpl; rewrite <- nth_error_Some, Hincl; discriminate.
+  - rewrite <- (sepcon_emp (ghost_hist _ _)).
+    apply sepcon_derives; auto.
+    apply andp_left2; auto.
+  - intros ?? Hin.
+    rewrite in_app in Hin; destruct Hin as [Hin | [X | ?]]; [| inv X | contradiction].
+    + specialize (Hincl _ _ Hin); rewrite nth_error_app1; auto.
+      rewrite <- nth_error_Some, Hincl; discriminate.
+    + rewrite nth_error_app2, minus_diag; auto.
+Qed.
